Further progress on parameterised relation
The idea seems to be working, but there is still more to do before I'm
certain. The basic idea is that the logical relation is parameterised by
a "world". The world maps locations (as would appear in an App SOME) to
location#arity#expression tuples. Closures with SOME annotations are
only related when the worlds expression is related to the closure's
expression, if the location of the SOME is present in the world
(otherwise there is no restriction). Furthermore, the code table must
hold an expression at the location of the world's range that is related
to the world's expression.

compiler/backend/semantics/clos_relationPropsScript.sml
@@ -289,8 +289,8 @@ val exp_rel_rtc_semantics_lem = Q.prove (
     ∀(s1:'ffi closSem$state) s2.
       (∀i. state_rel i w s1 s2) ∧ ¬(semantics [] s1 e1 = Fail) ⇒
        semantics [] s1 e1 = semantics [] s2 e2`,
- ho_match_mp_tac RTC_INDUCT >>
- metis_tac [exp_rel_semantics, state_rel_refl, exp_rel_refl]);
+ ho_match_mp_tac RTC_INDUCT
+ >> metis_tac [exp_rel_semantics, exp_rel_refl, state_rel_refl2]);
 
 val exp_rel_rtc_semantics = Q.store_thm(
   "exp_rel_rtc_semantics",
@@ -802,11 +802,57 @@ val exp_rel_thm = save_thm(
       |> SIMP_RULE (srw_ss() ++ DNF_ss) [exec_rel_rw, evaluate_ev_def,
                                          AND_IMP_INTRO]);
 
+val w_ok_def = Define `
+  w_ok w ⇔
+    !l l1 n1 e1 l2 n2 e2.
+      FLOOKUP w.code_restr l1 = SOME (l,n1,e1) ∧
+      FLOOKUP w.code_restr l2 = SOME (l,n2,e2)
+      ⇒
+      n1 = n2 ∧
+      e1 = e2`;
+
+val exists_ok_state = Q.store_thm ("exists_ok_state",
+  `!w i. w_ok w ⇒ ∃(s:'ffi closSem$state). state_ok i w s`,
+  rw [state_ok_def, FEVERY_DEF]
+  >> qexists_tac
+       `<| globals := ARB; refs := ARB; clock := ARB; ffi := ARB;
+           code := FUN_FMAP (\l. (@t. (l,t) ∈ (FRANGE w.code_restr))) (IMAGE FST (FRANGE w.code_restr))
+           |>`
+  >> rw []
+  >> pairarg_tac
+  >> simp [FLOOKUP_FUN_FMAP]
+  >> qexists_tac `e`
+  >> conj_tac
+  >- (
+    conj_asm1_tac
+    >- (
+      qexists_tac `(l',n,e)`
+      >> rw [IN_FRANGE]
+      >> metis_tac [])
+    >> irule SELECT_UNIQUE
+    >> strip_tac
+    >> eq_tac
+    >> rw []
+    >- (
+      PairCases_on `x'`
+      >> fs []
+      >> PairCases_on `y`
+      >> fs [w_ok_def, IN_FRANGE, FLOOKUP_DEF]
+      >> res_tac
+      >> rw [])
+    >> fs [IN_FRANGE]
+    >> metis_tac [])
+  >> rw []
+  >> `exp_rel (:'ffi) w [e] [e]` by metis_tac [exp_rel_refl]
+  >> fs [exp_rel_def]);
+
 val exp_rel_NIL_CONS = Q.store_thm(
   "exp_rel_NIL_CONS[simp]",
-  `exp_rel (:'ffi) w [] (e::es) ⇔ F`,
+  `w_ok w ⇒ (exp_rel (:'ffi) w [] (e::es) ⇔ F)`,
   simp[exp_rel_thm, evaluate_def] >>
   simp[Once evaluate_CONS, res_rel_rw, pair_case_eq, eqs] >>
+  rw [] >>
+  `?s i. state_ok i w (s : 'ffi closSem$state)` by metis_tac [exists_ok_state] >>
   metis_tac[val_rel_refl, state_rel_refl, DECIDE ``n:num ≤ n``]);
 
 val res_rel_Rerr_Rval = Q.store_thm(
@@ -834,7 +880,7 @@ val res_rel_cases = Q.store_thm(
        s1.clock = s2.clock) ∨
      (∃s1 s2. v1 = (Rerr (Rabort Rtimeout_error), s1) ∧
               v2 = (Rerr (Rabort Rtimeout_error), s2) ∧
-              state_rel s1.clock s1 s2)`,
+              state_rel s1.clock w s1 s2)`,
   Cases_on `v1` >> rename1 `res_rel _ (res1, s1)` >>
   Cases_on `v2` >> rename1 `res_rel _ _ (res2, s2)` >>
   Cases_on `res1` >> simp[] >> Cases_on `res2` >> simp[res_rel_rw]
@@ -858,12 +904,13 @@ val val_rel_bool = Q.store_thm(
   `val_rel (:'ffi) c w (Boolv b) v ⇔ v = Boolv b`,
   Cases_on `v` >> simp[val_rel_rw, Boolv_def] >> metis_tac[]);
 
- `exp_rel (:'ffi) w [f] [f'] ∧
+ `FLOOKUP w.code_restr loc = SOME (loc',n,e) ∧
+  exp_rel (:'ffi) w [f] [f'] ∧
   exp_rel (:'ffi) w es es'
   ⇒
   exp_rel (:'ffi) w
     [App (SOME loc) f es]
-    [Let (es'++[f']) (closLang$Call loc (MAP Var (COUNT_LIST (LENGTH es'))))]`,
+    [Let (es'++[f']) (closLang$Call loc' (MAP Var (COUNT_LIST (LENGTH es'))))]`,
 
   rw [exp_rel_thm]
   >> rw [evaluate_ev_def, evaluate_def]
@@ -886,8 +933,8 @@ val val_rel_bool = Q.store_thm(
   >> imp_res_tac evaluate_SING
   >> fs []
   >> rw []
-  >> qcase_tac `evaluate_app (SOME loc) fval args s3`
-  >> qcase_tac `evaluate (_, args' ++ [fval'] ++ env', s3')`
+  >> rename1 `evaluate_app (SOME loc) fval args s3`
+  >> rename1 `evaluate (_, args' ++ [fval'] ++ env', s3')`
   >> `LENGTH es' = LENGTH args' ∧ LENGTH es = LENGTH args` by cheat
   >> `LENGTH args = LENGTH args'` by metis_tac [LIST_REL_LENGTH, LESS_EQ_REFL]
   >> simp [evaluate_vars]
